updates

Jax/Jatlx.lean
@@ -1,29 +1,7 @@
-/- Layout of this File: -/
-/-
-  The user writes programs in a subset of the jaxpr language. Jaxpr expressions
-  are first preprocessed into ATL programs. Then ATL programs are normalized
-  into the SSA form. Operational semantics is defined for the SSA form of ATL.
-  After normalization, we just run the SSA form program based on the operational
-  semantics.
-
-  The file contains the following sections:
-  - Syntax of ATL in SSA form
-  - Functions for transforming jaxpr into ATL SSA form
-    (and jaxpr's syntax, which is just a few lines since
-     it's very similar to ATL)
-  - Operational semantics of ATL in SSA form
-    (including "built in" primitive functions for jaxpr implementd in ATL)
--/
-
-/- modifications to jax: 
-   - no named arguments for primitive functions, only simple let bindings,
-     only one variable on lhs, one expression on right
-   - 
--/
-
 /-************** ATL Syntax in Single-Static-Assignment Form *******************-/
+/- name, suffix for counting # calls, differentiation level, counter for use within autodiff -/
 inductive stmt_var
-| stmtV : String → Nat → stmt_var
+| stmtV : String → Nat → Nat → Nat → stmt_var
 /- since ATL is in normal form, index variables can be standardized into only 4 possible cases -/
 inductive ind_var
 | gen : Nat → ind_var
@@ -52,9 +30,18 @@ inductive binPrim
 | add
 | mult
 | sub
-| div
 inductive uniPrim
 | neg
+
+inductive ind_bound
+| const : Nat → ind_bound
+| var : stmt_var → Nat → ind_bound
+| max : ind_bound → ind_bound → ind_bound
+| add : ind_bound → ind_bound → ind_bound
+| mult : ind_bound → ind_bound → ind_bound
+| sub : ind_bound → ind_bound → ind_bound
+| div : ind_bound → ind_bound → ind_bound
+
 /- scalar expressions -/
 inductive exp  
 | const : Nat → exp
@@ -64,22 +51,18 @@ inductive exp
 | uniOp : 
   pred → uniPrim → stmt_var → exp
 | binTenSum : 
-  List Nat → List Nat → List Nat →
+  List ind_bound → List ind_bound → List ind_bound →
   pred → stmt_var → stmt_var → exp
 | uniTenSum :
-  List Nat → List Nat →
+  List ind_bound → List ind_bound →
   pred → stmt_var → exp
 
 inductive tenVal
 | val : List Nat → List Nat → tenVal
 
-inductive genIndBound
-| const : Nat → genIndBound
-| var : stmt_var → Nat → genIndBound
-| max : stmt_var → Nat → stmt_var → Nat → genIndBound
 /- tensor expession -/
 inductive unitTenExp  
-| gen : List genIndBound → exp → unitTenExp
+| gen : List ind_bound → exp → unitTenExp
 | var : stmt_var → unitTenExp
 | val : tenVal → unitTenExp
 inductive tenStmt
@@ -93,72 +76,87 @@ inductive tenExp
 inductive tenFunc 
 | func : List stmt_var → tenExp → tenFunc
 
-/-******************** Jaxpr and Lowering it to ATL ********************-/
-inductive jStmt
-| stmt : stmt_var → String → List stmt_var → jStmt
-| skip
-inductive jaxpr_body 
-| letList : List jStmt → stmt_var → jaxpr_body
-inductive jaxpr  
-| func : List stmt_var → jaxpr_body → jaxpr
-
-def subst_lst_gen paras args (suf : Nat) :=
-  match paras, args with
-  | [], _ => []
-  | _, [] => []
-  | (stmt_var.stmtV para _) :: rstparas, 
-    arg :: rstargs =>
-    (tenStmt.stmt (stmt_var.stmtV para suf) (unitTenExp.var arg)) :: 
-    subst_lst_gen rstparas rstargs suf
-def var_suf_set stVar suf :=
-  match stVar with
-  | stmt_var.stmtV var _ => stmt_var.stmtV var suf
-def exp_suf_update (suf : Nat) : exp → exp
-  | exp.const c => exp.const c
-  | exp.binOp p1 var1 op
-               p2 var2 =>
-    exp.binOp p1 (var_suf_set var1 suf) op
-               p2 (var_suf_set var2 suf)
-  | exp.uniOp p f var =>
-    exp.uniOp p f (var_suf_set var suf)
-  | exp.binTenSum indLst1 indLst2 indLst3
-                   p var1 var2 =>
-    exp.binTenSum indLst1 indLst2 indLst3 p
-                   (var_suf_set var1 suf) (var_suf_set var2 suf)
-  | exp.uniTenSum indLst1 indLst2 p var =>
-    exp.uniTenSum indLst1 indLst2 p (var_suf_set var suf)
-def suf_update suf 
-  | tenStmt.stmt varLHS (unitTenExp.var varRHS) =>
-    tenStmt.stmt (var_suf_set varLHS suf) (unitTenExp.var (var_suf_set varRHS suf))
-  | tenStmt.stmt svar (unitTenExp.gen indList e) =>
-    tenStmt.stmt (var_suf_set svar suf) (unitTenExp.gen indList (exp_suf_update suf e))
-  | tenStmt.stmt svar (unitTenExp.val val) =>
-    tenStmt.stmt svar (unitTenExp.val val)
-  | tenStmt.skip => tenStmt.skip
-def inline_prims stmts (env : String → tenFunc) (var_suf : Nat) :=
-  match stmts with
-  | [] => []
-  | jStmt.stmt target_var prim_name arg_vars :: rst =>
-    match env prim_name with
-    | tenFunc.func inp_vars (tenExp.letList fstmts (stmt_var.stmtV outName _)) =>
-      subst_lst_gen inp_vars arg_vars var_suf ++
-      (List.map (suf_update var_suf) fstmts) ++
-      tenStmt.stmt target_var (unitTenExp.var (stmt_var.stmtV outName var_suf)) ::
-        inline_prims rst env (1 + var_suf)
-  | jStmt.skip :: rst => tenStmt.skip :: inline_prims rst env var_suf
-/- transform a jaxpr into an ATL, by inlining primitives from environment -/
-def body_trans env body :=
-  match body with
-  | jaxpr_body.letList stmts out_var =>
-    tenExp.letList (inline_prims stmts env 1) out_var
-def jax_to_ATL p env :=
-  match p with
-  | jaxpr.func inp_vars body => 
-    tenFunc.func inp_vars (body_trans env body)
 
 /-********************* ATL Semantics in Single-Static-Assignment Form ********************-/
 /- given statement list and input environment, 
    return final environment after statements execute -/
+/- Helper Functions for Updating Statement Variable Environment -/
+def svar_env := stmt_var → tenVal
+def empty_senv : svar_env :=
+  fun _ => tenVal.val [] []
+def svar_eq
+  | stmt_var.stmtV str1 n1 n1' n1'', stmt_var.stmtV str2 n2 n2' n2'' =>
+    Bool.and (str1 == str2)
+      (Bool.and  (n1 == n2) (Bool.and (n1' == n2') (n1'' == n2'')))
+def update_senv {A} (env : stmt_var → A) (para : stmt_var) (arg : A) :=
+  fun x => if svar_eq x para then arg else env x
+def update_senv_star {A} (env : stmt_var → A) (paras : List stmt_var) (args : List A) :=
+  match paras, args with
+  | _, [] => env
+  | [], _ => env
+  | para :: paras', arg :: args' =>
+    update_senv_star (update_senv env para arg) paras' args'
+notation (name := senv_update) para:arg "!->s" arg:arg ";" env:arg =>
+  (update_senv env para arg)
+notation (name := senv_updates) paras:arg "!->s*" args:arg ";" env:arg =>
+  (update_senv_star env paras args)
+theorem svar_eq_trans_true :
+  ∀ var1 var2 var3,
+    svar_eq var1 var2 = true →
+    svar_eq var2 var3 = true →
+    svar_eq var1 var3 = true := by
+  intros var1 var2 var3 H1 H2
+  cases var1
+  case stmtV name1 n1 n1' n1'' =>
+  cases var2
+  case stmtV name2 n2 n2' n2'' =>
+  cases var3
+  case stmtV name3 n3 n3' n3'' =>
+  unfold svar_eq at *
+  simp at *
+  cases H1 with
+  | intro str12_eq n12_eq =>
+  cases n12_eq with
+  | intro n12_eq n12_eq' =>
+  cases n12_eq' with
+  | intro n12_eq' n12_eq'' =>
+  cases H2 with
+  | intro str23_eq n23_eq =>
+  cases n23_eq with
+  | intro n23_eq n23_eq' =>
+  cases n23_eq' with
+  | intro n23_eq' n23_eq'' =>
+  subst_vars
+  apply And.intro
+  rfl
+  apply And.intro
+  rfl
+  apply And.intro
+  rfl
+  rfl
+theorem svar_eq_trans_false :
+  ∀ var1 var2 var3,
+    svar_eq var1 var2 = false →
+    svar_eq var2 var3 = true →
+    svar_eq var1 var3 = false := by
+  intros var1 var2 var3 H1 H2
+  cases var1
+  case stmtV name1 n1 n1' n1'' =>
+  cases var2
+  case stmtV name2 n2 n2' n2'' =>
+  cases var3
+  case stmtV name3 n3 n3' n3'' =>
+  unfold svar_eq at *
+  simp at *
+  intro H_names H13 H13'
+  cases H2 with
+  | intro str23_eq n23_eq =>
+  cases n23_eq with
+  | intro n23_eq n23_eq' =>
+  cases n23_eq' with
+  | intro n23_eq' n23_eq'' =>
+  subst_vars
+  apply H1 <;> rfl
 
 /- Helper Functions for Updating Index Variable Environment -/
 def ivar_env := ind_var → Nat
@@ -177,31 +175,11 @@ def update_ienv_star env (paras : List ind_var) (args : List Nat) :=
   | [], _ => env
   | para :: paras', arg :: args' =>
     update_ienv_star (update_ienv env para arg) paras' args'
-/- https://www.leanprover.cn/mp-lean-zh/main/05_syntax.html -/
 notation (name := env_update) para:arg "!->i" arg:arg ";" env:arg =>
   (update_ienv env para arg)
 notation (name := env_updates) paras:arg "!->i*" args:arg ";" env:arg =>
   (update_ienv_star env paras args)
 
-/- Helper Functions for Updating Statement Variable Environment -/
-def svar_env := stmt_var → tenVal
-def empty_senv : svar_env :=
-  fun _ => tenVal.val [] []
-def svar_eq
-  | stmt_var.stmtV str1 n1, stmt_var.stmtV str2 n2 =>
-    Bool.and (str1 == str2) (n1 == n2)
-def update_senv {A} (env : stmt_var → A) (para : stmt_var) (arg : A) :=
-  fun x => if svar_eq x para then arg else env x
-def update_senv_star {A} (env : stmt_var → A) (paras : List stmt_var) (args : List A) :=
-  match paras, args with
-  | _, [] => env
-  | [], _ => env
-  | para :: paras', arg :: args' =>
-    update_senv_star (update_senv env para arg) paras' args'
-notation (name := senv_update) para:arg "!->s" arg:arg ";" env:arg =>
-  (update_senv env para arg)
-notation (name := senv_updates) paras:arg "!->s*" args:arg ";" env:arg =>
-  (update_senv_star env paras args)
 /- Helper Functions for Working with Indices and Predicates -/
 def ind_incr ivar :=
   match ivar with
@@ -270,27 +248,6 @@ def is_all_zeros
   | 0 :: lst' => is_all_zeros lst'
   | Nat.succ _ :: _ => false 
 
-
-/-
-def sum_2lst ind_lst1 ind_lst2 e env :=
-  let summand := (eval_var_acc e 
-  (var_lst1 !->i* ind_lst1; 
-  (var_lst2 !->i* ind_lst2; env)))
-  match is_all_zeros ind_lst1, is_all_zeros ind_lst2 with
-  | false, _ => summand + (sum_2lst (decr_lst ind_lst1) ind_lst2 e env)
-  | true, false => summand + (sum_2lst ind_lst1 (decr_lst ind_lst2) e env)
-  | true, true => summand
-def sum_3lst ind_lst1 ind_lst2 ind_lst3 e env :=
-  let summand := (eval_var_acc e 
-  (var_lst1 !->i* ind_lst1; 
-  (var_lst2 !->i* ind_lst2; 
-  (var_lst3 !->i* ind_lst3; env))))
-  match is_all_zeros ind_lst1, is_all_zeros ind_lst2, is_all_zeros ind_lst3 with
-  | false, _, _ => summand + (sum_3lst (decr_lst ind_lst1) ind_lst2 ind_lst3 e env)
-  | true, false, _ => summand + (sum_3lst ind_lst1 (decr_lst ind_lst2) ind_lst3 e env)
-  | true, true, false => summand + (sum_3lst ind_lst1 ind_lst2 (decr_lst ind_lst3) e env)
-  | true, true, true => summand
--/
 def ten_val_acc (shape : List Nat) (content : List Nat) (ind_lst : List Nat) begin_ptr end_ptr :=
   match shape, ind_lst with
   | [], [] => content.getD begin_ptr 0
@@ -310,7 +267,6 @@ def bin_op_app op (n1 n2 : Nat) :=
   | binPrim.add => n1 + n2
   | binPrim.sub => n1 - n2
   | binPrim.mult => n1 * n2
-  | binPrim.div => n1 / n2
 def uni_op_app op (n : Nat) :=
   match op with
   | uniPrim.neg => 0 - n
@@ -343,6 +299,43 @@ def sum_2tens sum_ind1 sum_ind2 sum_ind3 p var1 ind_acc1 var2 ind_acc2 senv ienv
 def iota 
   | 0 => []
   | Nat.succ n =>  (iota n) ++ [n]
+
+def eval_bound {X} (get_shape : (svar → X) → stmt_var → List Nat) env
+  | ind_bound.const n => n
+  | ind_bound.var name ind =>
+    (get_shape env name).getD ind 0 
+  | ind_bound.max arg1 arg2 =>
+    let n1 := eval_bound get_shape env arg1
+    let n2 := eval_bound get_shape env arg2
+    max n1 n2
+  | ind_bound.add arg1 arg2 =>
+    let n1 := eval_bound get_shape env arg1
+    let n2 := eval_bound get_shape env arg2
+    n1 + n2
+  | ind_bound.mult arg1 arg2 =>
+    let n1 := eval_bound get_shape env arg1
+    let n2 := eval_bound get_shape env arg2
+    n1 * n2
+  | ind_bound.sub arg1 arg2 =>
+    let n1 := eval_bound get_shape env arg1
+    let n2 := eval_bound get_shape env arg2
+    n1 - n2
+  | ind_bound.div arg1 arg2 =>
+    let n1 := eval_bound get_shape env arg1
+    let n2 := eval_bound get_shape env arg2
+    n1 / n2
+def get_shape_tm (senv : svar_env) var :=
+  match senv var with
+  | tenVal.val shape _ => shape
+
+def eval_shape {X} (get_shape : (svar → X) → stmt_var → List Nat) env
+  | [] => []
+  | some_bound :: rst_shape => 
+    (eval_bound get_shape env some_bound) 
+    :: (eval_shape get_shape env rst_shape)
+
+def eval_shape_tm env shape := eval_shape get_shape_tm env shape
+
 def eval_exp (senv : svar_env) (ienv : ivar_env) (gen_ind_acc : List ind_var) : exp → Nat
   | exp.const c => c
   | exp.binOp p1 var1 op p2 var2 =>
@@ -357,34 +350,23 @@ def eval_exp (senv : svar_env) (ienv : ivar_env) (gen_ind_acc : List ind_var) : 
     if eval_pred_bool p ienv
     then uni_op_app f (access senv ienv var gen_ind_acc)
     else 0
-  | exp.binTenSum n0 n1 ns p var0 var1 =>
+  | exp.binTenSum ind_lst0 ind_lst1 ind_lst_s p var0 var1 =>
+    let n0 := eval_shape_tm senv ind_lst0
+    let n1 := eval_shape_tm senv ind_lst1
+    let ns := eval_shape_tm senv ind_lst_s
     let ind_acc0 := List.map ind_var.sums (iota (List.length n0))
     let ind_acc1 := List.map ind_var.sum1 (iota (List.length n1))
     sum_2tens n0 n1 ns p var0 ind_acc0 var1 ind_acc1 senv ienv
-  | exp.uniTenSum n nS p var =>
+  | exp.uniTenSum ind_lst ind_lst_s p var =>
+    let n := eval_shape_tm senv ind_lst
+    let ns := eval_shape_tm senv ind_lst_s
     let ind_acc := List.map ind_var.sums (iota (List.length n))
-    sum_1tens n nS p var ind_acc senv ienv
+    sum_1tens n ns p var ind_acc senv ienv
     
 /- Evaluating Tensor Expressions -/
-/-  
-/- environment gives 0 by default, so shape list can be shrunk and information not lost-/
-def gen_tensor_h (shape counter : List Nat) (e : exp) senv ienv :=
-  let element := (eval_exp senv ((gen_ind_lst (List.length counter)) !->i* counter; ienv) e)
-  match counter with
-  | [] => [element]
-  | 0 :: lst' => gen_tensor_h shape lst' e senv ienv
-  | Nat.succ n :: lst' => 
-    (gen_tensor_h shape (n :: lst') e senv ienv) ++ [element]
-  
-/- turn the last index to front -/
-def gen_tensor shape e senv := 
-  tenVal.TVal shape (gen_tensor_h (List.reverse shape) (List.reverse shape) e senv empty_ienv)
--/
-
 def gen_ind_lst
   | 0 => []
   | Nat.succ n =>  (gen_ind_lst n) ++ [ind_var.gen n]
-
 /- gen tensor is gen list applied many times-/
 def gen_tensor_h (shape : List Nat) e senv ienv cur_ind (gen_ind_lst : List ind_var) :=
   match shape with
@@ -402,20 +384,7 @@ where gen_list cur_ind_var length (e : exp) (ienv : ivar_env)
 def gen_tensor shape e senv := 
   let gen_ind_lst := List.map ind_var.gen (iota (List.length shape))
   tenVal.val shape (gen_tensor_h shape e senv empty_ienv (ind_var.gen 0) gen_ind_lst)
-def get_shape_tm (senv : svar_env) var :=
-  match senv var with
-  | tenVal.val shape _ => shape
 
-def eval_shape {X} (get_shape : (svar → X) → stmt_var → List Nat) env
-  | [] => []
-  | genIndBound.const n :: rst_shape => n :: (eval_shape get_shape env rst_shape)
-  | genIndBound.var name ind :: rst_shape =>
-    (get_shape env name).getD ind 0 :: (eval_shape get_shape env rst_shape)
-  | genIndBound.max name1 ind1 name2 ind2 :: rst_shape =>
-    let n1 := (get_shape env name1).getD ind1 0
-    let n2 := (get_shape env name2).getD ind2 0
-    max n1 n2 :: (eval_shape get_shape env rst_shape)
-def eval_shape_tm env shape := eval_shape get_shape_tm env shape
 def eval_texp e senv := 
   match e with
   | unitTenExp.gen shape e' =>
@@ -435,14 +404,18 @@ def eval_stmts (env : svar_env) :
   | tenStmt.skip :: rst_stmts =>
     eval_stmts env rst_stmts
 
-def eval_prog prog args fenv :=
-  match jax_to_ATL prog fenv with
-  | tenFunc.func inp_vars (tenExp.letList stmts out) =>
-    (eval_stmts (inp_vars !->s* args ; empty_senv) stmts) out
-/- ************ Small Step Operational Semantics ************* -/
+def eval_ATL_body init_env
+  | tenExp.letList stmts out =>
+    (eval_stmts init_env stmts, out)
+def eval_ATL args
+  | tenFunc.func inp_vars expr =>
+    match eval_ATL_body (inp_vars !->s* args ; empty_senv) expr with
+    | (final_env, out) => final_env out
+
+/- ************ ATL Small Step Operational Semantics ************* -/
 inductive step_stmt : svar_env × tenStmt →
                       svar_env × tenStmt → Prop where
-| stp_stmt : ∀ env var exp,
+| stp_stmt : ∀ env var exp val,
   val = eval_texp exp env →
   new_env = var !->s val ; env →
   step_stmt (env, (tenStmt.stmt var exp)) (new_env, tenStmt.skip)
@@ -458,20 +431,134 @@ inductive step_fun_body : svar_env × tenExp →
 | stp_letList : ∀ env new_env stmts new_stmts out,
   step_stmts (env,stmts) (new_env, new_stmts) →
   step_fun_body (env, tenExp.letList stmts out) (new_env, tenExp.letList new_stmts out)
-/-
-take a program and get an absmachine initial state is not
-part of stepping semantics
+inductive step_fun_body_star : svar_env × tenExp →
+                               svar_env × tenExp → Prop where
+| no_stp : ∀ env tm, step_fun_body_star (env, tm) (env, tm)
+| stps  : ∀ env tm env' tm' env'' tm'', 
+  step_fun_body (env, tm) (env', tm') →
+  step_fun_body_star (env', tm') (env'', tm'') →
+  step_fun_body_star (env, tm) (env'', tm'')
 
-inductive steps_prog prog args fenv result
-| stps_prog : ∀ inp_vars stmts out final_env,
-  jax_to_ATL prog fenv = tenFunc.func inp_vars (tenExp.letList stmts out) →
-  steps_stmts (inp_vars !->s* args ; empty_senv) stmts final_env →
-  final_env out = result →
-  steps_prog prog args fenv result-/
-/- ************* Type System & Soundness Proof *************** -/
+/- ************* Proof that Small Step Correctly Simulates Denotational *************** -/
+
+theorem small_sim_deno : ∀ env env' expr out,
+  eval_ATL_body env expr = (env', out) →
+  step_fun_body_star (env, expr) (env', tenExp.letList [] out) := by
+  intros env env' expr out
+  intro H
+  cases expr with
+  | letList stmts out' =>
+  cases H
+  revert env
+  induction stmts with
+  | nil => 
+    intro env 
+    apply step_fun_body_star.no_stp
+  | cons head tail IH =>
+  cases head with
+  | skip =>
+    intro env
+    apply step_fun_body_star.stps
+    apply step_fun_body.stp_letList
+    . apply step_stmts.stp_skip
+    . unfold eval_stmts; apply IH
+  | stmt var exp =>
+    intro env
+    apply step_fun_body_star.stps
+    apply step_fun_body.stp_letList
+    . apply step_stmts.stp_stmts
+      apply step_stmt.stp_stmt <;> rfl
+    . apply step_fun_body_star.stps
+      apply step_fun_body.stp_letList
+      . apply step_stmts.stp_skip
+      . unfold eval_stmts
+        simp
+        apply IH
+
+theorem deno_sim_small : ∀ env env' expr out,
+  step_fun_body_star (env, expr) (env', tenExp.letList [] out) →
+  eval_ATL_body env expr = (env', out) := by
+  intros env env' expr out
+  intro H
+  unfold eval_ATL_body
+  cases expr with
+  | letList stmts out' =>
+  simp
+  apply And.intro
+  case right =>
+    revert env
+    induction stmts with
+    | nil => 
+      intro env H
+      cases H
+      . rfl
+      case stps env' tm' H_one_stp H_stps =>
+        cases H_one_stp
+        case stp_letList stmts H_stmts =>
+        cases H_stmts
+    | cons head tail IH =>
+      intro env H
+      cases H
+      case stps env_mid tm' H_one_stp H_stps =>
+      cases H_one_stp
+      case stp_letList stmts H_stmts =>
+      cases H_stmts
+      . have IH' := IH env H_stps
+        apply IH'
+      case stp_stmts new_stmt H_stmt =>
+        cases H_stmt
+        case stp_stmt env var exp val =>
+        subst_vars
+        cases H_stps
+        case stps env_mid tm' H_one_stp H_stps =>
+        cases H_one_stp
+        case stp_letList stmts H_stmts =>
+        cases H_stmts 
+        . apply IH
+          apply H_stps
+        case stp_stmts new_stmt H_stmt =>
+        cases H_stmt
+  case left =>
+    revert env
+    induction stmts with
+    | nil => 
+      intro env H
+      cases H
+      . rfl
+      case stps env' tm' H_one_stp H_stps =>
+        cases H_one_stp
+        case stp_letList stmts H_stmts =>
+        cases H_stmts
+    | cons head tail IH =>
+      intro env H
+      cases H
+      case stps env_mid tm' H_one_stp H_stps =>
+      cases H_one_stp
+      case stp_letList stmts H_stmts =>
+      cases H_stmts
+      . have IH' := IH env H_stps
+        apply IH'
+      case stp_stmts new_stmt H_stmt =>
+        cases H_stmt
+        case stp_stmt env var exp val =>
+        subst_vars
+        cases H_stps
+        case stps env_mid tm' H_one_stp H_stps =>
+        cases H_one_stp
+        case stp_letList stmts H_stmts =>
+        cases H_stmts 
+        . apply IH
+          apply H_stps
+        case stp_stmts new_stmt H_stmt =>
+        cases H_stmt
+
+theorem small_deno_agree : ∀ env env' expr out,
+  step_fun_body_star (env, expr) (env', tenExp.letList [] out) iff
+  eval_ATL_body env expr = (env', out) := by
+/- ************* ATL Type System & Soundness Proof *************** -/
 /- ************* Type Syntax *************** -/
 inductive ty_unitTenExp  
-| gen : List genIndBound → ty_unitTenExp
+| gen : List ind_bound → ty_unitTenExp
 | val : List Nat → ty_unitTenExp
 | var : stmt_var → ty_unitTenExp
 
@@ -489,15 +576,6 @@ inductive ty_tenFunc
 inductive ty_tenVal
 | val : List Nat → ty_tenVal
 
-inductive ty_jStmt
-| stmt : stmt_var → String → List stmt_var → ty_jStmt
-| skip
-
-inductive ty_jaxpr_body 
-| letList : List ty_jStmt → stmt_var → ty_jaxpr_body
-
-inductive ty_jaxpr  
-| func : List stmt_var → ty_jaxpr_body → ty_jaxpr
 /- ************* Small Step Type Reduction *************** -/
 /- type environment -/
 def ty_env := stmt_var → ty_tenVal
@@ -512,6 +590,86 @@ def get_shape_ty (senv : ty_env) var :=
   match senv var with
   | ty_tenVal.val shape => shape
 def eval_shape_ty env shape := eval_shape get_shape_ty env shape
+
+theorem lift_env_same_shape : ∀ env x,
+  (env x).1 = (lift_senv env x).1 := by
+  intros env x
+  unfold lift_senv
+  simp
+theorem eval_shape_lift_eq : ∀ env shape,
+  eval_shape_tm env shape = eval_shape_ty (lift_senv env) shape := by
+  intros env shape
+  induction shape with
+  | nil => rfl
+  | cons head tail IH =>
+    unfold eval_shape_tm eval_shape_ty
+    unfold eval_shape get_shape_tm get_shape_ty
+    simp
+    induction head with
+    | const n => 
+      apply And.intro
+      . unfold eval_bound ; rfl
+      . apply IH      
+    | var name suffix =>
+      apply And.intro
+      . unfold eval_bound; rfl
+      . apply IH
+    | max arg1 arg2 IH1 IH2 =>
+      cases IH1 with
+      | intro IH1 IH_tail =>
+      cases IH2 with
+      | intro IH2 IH_tail =>
+      apply And.intro
+      . unfold eval_bound
+        rewrite [IH1]
+        rewrite [IH2]
+        rfl
+      . apply IH_tail
+    | add arg1 arg2 IH1 IH2 =>
+      cases IH1 with
+      | intro IH1 IH_tail =>
+      cases IH2 with
+      | intro IH2 IH_tail =>
+      apply And.intro
+      . unfold eval_bound
+        rewrite [IH1]
+        rewrite [IH2]
+        rfl
+      . apply IH_tail
+    | mult arg1 arg2 IH1 IH2 =>
+      cases IH1 with
+      | intro IH1 IH_tail =>
+      cases IH2 with
+      | intro IH2 IH_tail =>
+      apply And.intro
+      . unfold eval_bound
+        rewrite [IH1]
+        rewrite [IH2]
+        rfl
+      . apply IH_tail
+    | sub arg1 arg2 IH1 IH2 =>
+      cases IH1 with
+      | intro IH1 IH_tail =>
+      cases IH2 with
+      | intro IH2 IH_tail =>
+      apply And.intro
+      . unfold eval_bound
+        rewrite [IH1]
+        rewrite [IH2]
+        rfl
+      . apply IH_tail
+    | div arg1 arg2 IH1 IH2 =>
+      cases IH1 with
+      | intro IH1 IH_tail =>
+      cases IH2 with
+      | intro IH2 IH_tail =>
+      apply And.intro
+      . unfold eval_bound
+        rewrite [IH1]
+        rewrite [IH2]
+        rfl
+      . apply IH_tail
+
 def eval_ty_texp (senv : ty_env) 
   | ty_unitTenExp.val shape =>
     ty_tenVal.val shape
@@ -541,8 +699,8 @@ inductive ty_step_fun_body_star : ty_env × ty_tenExp →
                                   ty_env × ty_tenExp → Prop where
 | no_stp : ∀ env ty, ty_step_fun_body_star (env, ty) (env, ty)
 | stps  : ∀ env ty env' ty' env'' ty'', 
-  ty_step_fun_body_star (env, ty) (env', ty') →
-  ty_step_fun_body (env', ty') (env'', ty'') →
+  ty_step_fun_body (env, ty) (env', ty') →
+  ty_step_fun_body_star (env', ty') (env'', ty'') →
   ty_step_fun_body_star (env, ty) (env'', ty'')
 /- ************* Typing Rules *************** -/
 inductive has_ty_unitTenExp : unitTenExp → ty_unitTenExp → Prop where
@@ -559,6 +717,7 @@ inductive has_ty_unitTenExp : unitTenExp → ty_unitTenExp → Prop where
   val_ty = ty_unitTenExp.val shape →
   has_ty_unitTenExp val_tm val_ty
 inductive has_ty_tenStmt : tenStmt → ty_tenStmt → Prop where
+| skip : has_ty_tenStmt tenStmt.skip ty_tenStmt.skip
 | stmt : ∀ stmt_tm stmt_ty var_tm var_ty exp_tm exp_ty,
   stmt_tm = tenStmt.stmt var_tm exp_tm →
   stmt_ty = ty_tenStmt.stmt var_ty exp_ty →
@@ -598,11 +757,318 @@ inductive has_ty_tenVal : tenVal → ty_tenVal → Prop where
   val_tm = tenVal.val shape content →
   val_ty = ty_tenVal.val shape →
   has_ty_tenVal val_tm val_ty
+
+inductive is_terminal : tenExp → Prop where
+| is_term : ∀ tm out,
+  tm = tenExp.letList [] out →
+  is_terminal tm
+
+inductive ty_is_terminal : ty_tenExp → Prop where
+| is_term : ∀ ty out,
+  ty = ty_tenExp.letList [] out →
+  ty_is_terminal ty
+
+def unstuck tm env :=
+  is_terminal tm ∨
+  ∃ env' tm', step_fun_body (env, tm) (env', tm')
+def ty_eq env1 ty1 env2 ty2 :=
+  ty_step_fun_body_star (env1, ty1) (env2, ty2) ∨
+  ty_step_fun_body_star (env2, ty2) (env1, ty1)
+
+theorem ty_step_fun_body_star_concat : ∀ env ty env' ty' env'' ty'',
+  ty_step_fun_body_star (env, ty) (env', ty') →
+  ty_step_fun_body_star (env', ty') (env'', ty'') →
+  ty_step_fun_body_star (env, ty) (env'', ty'') := by
+  intros env ty env' ty' env'' ty'' H_steps1 H_steps2
+  generalize H1 : (env, ty) = pair1
+  generalize H2 : (env', ty') = pair2
+  rw [H1, H2] at H_steps1
+  revert ty ty ty' env env' env'' ty''
+  induction H_steps1 with
+  | no_stp env ty =>
+    intros env1 ty1 env' ty' env'' ty'' H_steps2 H1 H2
+    cases H1
+    cases H2
+    apply H_steps2
+  | stps env ty env' ty' env'' ty'' H_stp_one H_stps_star IH =>
+    intros env1 ty1 env''1 ty''1 env''' ty''' H_steps2 H1 H2
+    cases H1
+    cases H2
+    have IH' := IH env' ty' env'' ty'' env''' ty''' H_steps2 rfl rfl
+    apply ty_step_fun_body_star.stps
+    . apply H_stp_one
+    . apply IH'
+
+/- ************* Type Soundness *************** -/
+
+theorem progress : ∀ tm env ty,
+  has_ty_tenExp tm ty → unstuck tm env := by
+  intros tm env ty H
+  cases tm with
+  | letList stmts out =>
+    cases stmts
+    . apply Or.inl; apply is_terminal.is_term ; rfl
+    case cons stmt rst_stmts => 
+      apply Or.inr
+      cases stmt
+      case skip => 
+        exists env, tenExp.letList rst_stmts out
+        apply step_fun_body.stp_letList
+        apply step_stmts.stp_skip
+      case stmt var exp =>
+        exists var !->s (eval_texp exp env) ; env
+        exists tenExp.letList (tenStmt.skip :: rst_stmts) out
+        apply step_fun_body.stp_letList
+        apply step_stmts.stp_stmts
+        apply step_stmt.stp_stmt
+        . rfl
+        . rfl
+
+theorem preservation_strong : ∀ tm env tm' env' ty,
+  has_ty_tenExp tm ty →
+  step_fun_body (env, tm) (env', tm') →
+  ∃ ty', 
+    has_ty_tenExp tm' ty' ∧
+    ty_step_fun_body_star (lift_senv env, ty) (lift_senv env', ty') := by
+  intros tm env tm' env' ty H_ty H_step
+  cases H_step with
+  | stp_letList env env' stmts stmts' out H_stp_stmts =>
+  cases H_stp_stmts with
+  | stp_skip env some_stmts => 
+    cases H_ty with
+    | letList letList_tm letList_ty out_tm out_ty
+              H_tm H_ty H_var_eq H_stmts_ty =>
+      subst_vars
+      cases H_tm
+      cases letList_ty with
+      | nil => contradiction
+      | cons stmt_ty rst_stmts_ty =>
+      exists (ty_tenExp.letList rst_stmts_ty out_ty)
+      cases H_stmts_ty with
+      | intro left right =>
+      apply And.intro
+      . apply has_ty_tenExp.letList <;> try rfl
+        apply H_var_eq
+        apply right
+      . apply ty_step_fun_body_star.stps
+        . cases left
+          . apply ty_step_fun_body.stp_letList
+            apply ty_step_stmts.stp_skip
+          . contradiction
+        . apply ty_step_fun_body_star.no_stp
+  | stp_stmts env env' stmt new_stmt some_stmts H_stp_stmt => 
+    cases H_ty with
+    | letList letList_tm letList_ty out_tm out_ty
+              H_tm H_ty H_var_eq H_stmts_ty =>
+      subst_vars
+      cases H_tm
+      cases letList_ty with
+      | nil => contradiction
+      | cons stmt_ty rst_stmts_ty =>
+      cases H_stmts_ty with
+      | intro left right =>
+      cases H_stp_stmt with
+      | stp_stmt env var exp val H_val H_env =>
+      subst_vars
+      exists (ty_tenExp.letList (ty_tenStmt.skip :: rst_stmts_ty) out_ty)
+      apply And.intro
+      . apply has_ty_tenExp.letList <;> try rfl
+        apply H_var_eq
+        unfold has_ty_stmtLst
+        apply And.intro
+        apply has_ty_tenStmt.skip
+        apply right
+      . apply ty_step_fun_body_star.stps <;> try (apply ty_step_fun_body_star.no_stp)
+        cases left with
+        | stmt stmt_tm stmt_ty var_tm var_ty exp_tm exp_ty
+               H_tm H_ty H_var_eq' H_unitTen =>
+          apply ty_step_fun_body.stp_letList
+          apply ty_step_stmts.stp_stmts
+          subst_vars
+          apply ty_step_stmt.stp_stmt <;> try rfl
+          unfold lift_senv update_senv
+          funext x
+          simp
+          cases H_tm
+          cases eqn : (svar_eq x var)
+          . rewrite [svar_eq_trans_false]
+            simp
+            apply var
+            apply eqn
+            apply H_var_eq'
+          . rewrite [svar_eq_trans_true] 
+            . simp
+              cases H_unitTen <;> subst_vars <;> unfold eval_texp <;> 
+                unfold eval_ty_texp <;> simp
+              case a.stmt.a.a.a.h.refl.true.gen shape e =>
+                unfold gen_tensor
+                simp
+                apply eval_shape_lift_eq
+            . apply var
+            . apply eqn
+            . apply H_var_eq'
+        
+theorem preservation : ∀ tm env tm' env' ty,
+  has_ty_tenExp tm ty →
+  step_fun_body (env, tm) (env', tm') →
+  ∃ ty', 
+    has_ty_tenExp tm' ty' ∧
+    ty_eq (lift_senv env) ty (lift_senv env') ty' := by
+  intros tm env tm' env' ty H_ty H_step
+  have H := preservation_strong tm env tm' env' ty H_ty H_step
+  cases H with
+  | intro ty' H =>
+  cases H with
+  | intro left right =>
+  exists ty'
+  apply And.intro
+  . apply left
+  . unfold ty_eq
+    apply Or.inl
+    apply right
+
+theorem type_safety_h : ∀ tm1 env1 tm2 env2 ty1,
+  has_ty_tenExp tm1 ty1 →
+  step_fun_body_star (env1, tm1) (env2, tm2) →
+  ∃ ty2,
+    has_ty_tenExp tm2 ty2 ∧
+    ty_step_fun_body_star (lift_senv env1, ty1) (lift_senv env2, ty2) := by
+  intros tm1 env1 tm2 env2 ty H_has_ty H_steps 
+  generalize H1 : (env1, tm1) = pair1
+  rw [H1] at H_steps
+  generalize H2 : (env2, tm2) = pair2
+  rw [H2] at H_steps
+  revert ty tm1 tm2 env1 env2
+  induction H_steps with
+  | no_stp env tm =>
+    intro tm1 env1 tm2 env2 ty H_has_ty H_p1 H_p2
+    cases H_p1
+    cases H_p2
+    exists ty
+    apply And.intro
+    . apply H_has_ty
+    . apply ty_step_fun_body_star.no_stp
+  | stps env tm env' tm' env'' tm'' H_stp_one H_stps_star IH =>
+    intro tm1 env1 tm2 env2 ty H_has_ty H_p1 H_p2
+    cases H_p1
+    cases H_p2
+    
+    have H_pres := preservation_strong tm env tm' env' ty H_has_ty H_stp_one
+    cases H_pres with
+    | intro ty1 H_pres =>
+    cases H_pres with
+    | intro H_pres1 H_pres2 =>
+    have IH' := IH tm' env' tm'' env'' ty1 H_pres1 rfl rfl
+    cases IH' with
+    | intro ty2 IH =>
+    cases IH with
+    | intro IH1 IH2 =>
+    exists ty2
+    apply And.intro
+    . apply IH1
+    . apply ty_step_fun_body_star_concat
+      apply H_pres2
+      apply IH2 
+
+theorem type_safety : ∀ tm1 env1 tm2 env2 ty,
+  has_ty_tenExp tm1 ty →
+  step_fun_body_star (env1, tm1) (env2, tm2) →
+  unstuck tm2 env2 := by
+  intros tm1 env1 tm2 env2 ty H_has_ty H_steps 
+  have H := type_safety_h tm1 env1 tm2 env2 ty H_has_ty H_steps
+  cases H with
+  | intro ty2 H =>
+  cases H with
+  | intro left right =>
+  apply progress
+  apply left
+
+/-************************ Forward Mode Autodiff on ATL ***********************-/
+def var_diff
+  | stmt_var.stmtV name suf diff_level diff_counter =>
+    stmt_var.stmtV name suf (Nat.succ diff_level) diff_counter
+def diff_temp_gen
+  | stmt_var.stmtV name suf diff_level diff_counter =>
+    stmt_var.stmtV name suf diff_level (Nat.succ diff_counter)
+def forward_diff_exp target_var shape expr :=
+  let stmt_wrapper_h the_var x := tenStmt.stmt (var_diff the_var)
+                                               (unitTenExp.gen shape x)
+  let stmt_wrapper x := stmt_wrapper_h target_var x
+  let temp1 := diff_temp_gen target_var
+  let temp2 := diff_temp_gen temp1
+  match expr with
+  | exp.const _ => [stmt_wrapper (exp.const 0)]
+  | exp.binOp pred1 var1 binPrim.add pred2 var2 =>
+    [stmt_wrapper (exp.binOp pred1 (var_diff var1) binPrim.add pred2 (var_diff var2))]
+  | exp.binOp pred1 var1 binPrim.sub pred2 var2 =>
+    [stmt_wrapper (exp.binOp pred1 (var_diff var1) binPrim.sub pred2 (var_diff var2))]
+  | exp.binOp pred1 var1 binPrim.mult pred2 var2 =>
+    stmt_wrapper_h temp1 (exp.binOp pred1 (var_diff var1) binPrim.mult pred2 var2) ::
+    stmt_wrapper_h temp2 (exp.binOp pred1 var1 binPrim.mult pred2 (var_diff var2)) ::
+    [stmt_wrapper (exp.binOp pred1 temp1 binPrim.add pred2 temp2)]
+  | exp.uniOp p uniPrim.neg var =>
+    [stmt_wrapper (exp.uniOp p uniPrim.neg (var_diff var))]
+  | exp.binTenSum bound_lst1 bound_lst2 bound_lst_s
+                  p var1 var2 =>
+    stmt_wrapper_h temp1 
+      (exp.binTenSum bound_lst1 bound_lst2 bound_lst_s p (var_diff var1) var2) ::
+    stmt_wrapper_h temp2 
+      (exp.binTenSum bound_lst1 bound_lst2 bound_lst_s p var1 (var_diff var2)) ::
+    [stmt_wrapper (exp.binOp pred.true temp1 binPrim.add pred.true temp2)]
+  | exp.uniTenSum bound_lst1 bound_lst2 p var =>
+    [stmt_wrapper (exp.uniTenSum bound_lst1 bound_lst2 p (var_diff var))]
+       
+def forward_diff_tenExp target_var
+  | unitTenExp.var var => 
+    [tenStmt.stmt (var_diff target_var) (unitTenExp.var (var_diff var))]
+  | unitTenExp.val (tenVal.val shape content) =>
+    [tenStmt.stmt (var_diff target_var) 
+      (unitTenExp.val (tenVal.val shape (List.map (fun _ => 0) content)))]
+  | unitTenExp.gen shape exp =>
+    forward_diff_exp target_var shape exp
+/- solve the issue by using return type list -/
+def forward_diff_stmt_lst env
+  | [] => []
+  | tenStmt.skip :: rst => forward_diff_stmt_lst env rst
+  | tenStmt.stmt var exp :: rst =>
+    let new_env := var !->s (var_diff var) ; env
+    tenStmt.stmt var exp ::
+    forward_diff_tenExp var exp ++
+    forward_diff_stmt_lst new_env rst
+def forward_diff
+  | tenFunc.func inp_vars (tenExp.letList stmts out) =>
+    let empty_var_env := fun _ => stmt_var.stmtV "" 0 0 0
+    tenFunc.func inp_vars (tenExp.letList (forward_diff_stmt_lst empty_var_env stmts) out)
+def forward_many_diff expr
+  | 0 => expr
+  | Nat.succ n => forward_many_diff (forward_diff expr) n
+
+/-******************** Jaxpr and Lowering it to ATL ********************-/
+inductive jStmt
+| stmt : stmt_var → String → Nat → List stmt_var → jStmt
+| skip
+inductive jaxpr_body 
+| letList : List jStmt → stmt_var → jaxpr_body
+inductive jaxpr  
+| func : List stmt_var → jaxpr_body → jaxpr
+
+/- *********** Jax Type System ****************** -/
+
+inductive ty_jStmt
+| stmt : stmt_var → String → Nat → List stmt_var → ty_jStmt
+| skip
+
+inductive ty_jaxpr_body 
+| letList : List ty_jStmt → stmt_var → ty_jaxpr_body
+
+inductive ty_jaxpr  
+| func : List stmt_var → ty_jaxpr_body → ty_jaxpr
+
 inductive has_ty_jStmt : jStmt → ty_jStmt → Prop where
 | stmt : ∀ stmt_tm stmt_ty var_tm var_ty 
-           prim_tm prim_ty args_tm args_ty,
-  stmt_tm = jStmt.stmt var_tm prim_tm args_tm →
-  stmt_ty = ty_jStmt.stmt var_ty prim_ty args_ty →
+           prim_tm prim_ty args_tm args_ty diff_tm diff_ty,
+  stmt_tm = jStmt.stmt var_tm prim_tm diff_tm args_tm →
+  stmt_ty = ty_jStmt.stmt var_ty prim_ty diff_ty args_ty →
   svar_eq var_tm var_ty = true →
   (prim_tm == prim_ty) = true →
   svar_lst_eq args_tm args_ty →
@@ -632,169 +1098,148 @@ inductive has_ty_jaxpr : jaxpr → ty_jaxpr → Prop where
   has_ty_jaxpr_body body_tm body_ty →
   has_ty_jaxpr func_tm func_ty
 
-inductive is_terminal : tenExp → Prop where
-| is_term : ∀ tm out,
-  tm = tenExp.letList [] out →
-  is_terminal tm
 
-def ty_eq env1 ty1 env2 ty2 :=
-  ∃ env ty, 
-  ty_step_fun_body_star (env1, ty1) (env, ty) ∧
-  ty_step_fun_body_star (env2, ty2) (env, ty)
-/-
-inductive has_type_atl : tenFunc → ty → Prop where
-| T_atl : ∀ body inp_shapes, 
-  type_of_free_vars body = inp_shapes →
-  has_type_atl_body body out_shapes →
-  has_type_atl 
-    (tenFunc.TFunc inp_vars body)
-    (func_ty inp_shapes out_shapes)
-inductive has_type_j_body
-inductive has_type_j : jaxpr → ty → Prop where
-| T_prog : ∀ jbody inp_shapes, 
-  type_of_free_vars jbody = inp_shapes →
-  has_type_jbody jbody out_shapes →
-  has_type_j 
-    (jaxpr.func inp_vars jbody)
-    (func_ty inp_shapes out_shapes) -/
-/- type abs and app for shapes and ranks -/
-/- function type should give info for how to compute a shape when given a list of shapes -/
-/- shapes of inputs and shape of output -/
-/-
-inductive ty 
-| func_ty : List (List Nat) → List Nat → ty
-| val_ty : List Nat → ty
-def type_of_free_vars seen_vars : List (stmt_var × String × List stmt_var) → List (List Nat)
-  | jaxpr_body.JLetList [] out => []
-  | jaxpr_body.JLetList ((var, prim_func, arg_lst) :: stmt_lst) out =>
-    if List.filter seen_vars arg_lst = []
-    type_of_free_vars stmt_lst
+/- ***** lowering to ATL ***** -/
+def var_suf_incr stVar suf :=
+  match stVar with
+  | stmt_var.stmtV var original_suf diff count => 
+    stmt_var.stmtV var (suf + original_suf) diff count
 
-    
-theorem progress : eval_prog simple_prog [arg1,arg2,arg3] prim_env = 
-             tenVal.TVal [2,2] [8, 9, 8, 9] := by simp-/
-/- ************* Type Soundness *************** -/
+def subst_lst_gen paras args (suf : Nat) :=
+  match paras, args with
+  | [], _ => []
+  | _, [] => []
+  | var :: rstparas, 
+    arg :: rstargs =>
+    (tenStmt.stmt (var_suf_incr var suf) (unitTenExp.var arg)) :: 
+    subst_lst_gen rstparas rstargs suf
 
-theorem progress : ∀ tm env ty,
-  has_ty_tenExp tm ty →
-  is_terminal tm ∨
-  ∃ env' tm', step_fun_body (env, tm) (env', tm') := by
-  intros tm env ty H
-  cases tm with
-  | letList stmts out =>
-    cases stmts
-    . apply Or.inl; apply is_terminal.is_term ; rfl
-    case cons stmt rst_stmts => 
-      apply Or.inr
-      cases stmt
-      case skip => 
-        exists env, tenExp.letList rst_stmts out
-        apply step_fun_body.stp_letList
-        apply step_stmts.stp_skip
-      case stmt var exp =>
-        exists var !->s (eval_texp exp env) ; env
-        exists tenExp.letList (tenStmt.skip :: rst_stmts) out
-        apply step_fun_body.stp_letList
-        apply step_stmts.stp_stmts
-        apply step_stmt.stp_stmt
-        . rfl
-        . rfl
-  
-theorem preservation : ∀ tm env tm' env' ty,
-  step_fun_body (env, tm) (env', tm') →
-  has_ty_tenExp tm ty →
-  ∃ ty', 
-    has_ty_tenExp tm' ty' ∧
-    ty_eq (lift_senv env) ty (lift_senv env') ty' := by
-  intros tm env tm' env' ty H_step H_ty
-  cases H_step with
-  | stp_letList env env' stmts stmts' out H_stp_stmts =>
-  cases H_stp_stmts with
-  | stp_skip env some_stmts => 
-    cases H_ty with
-    | letList letList_tm letList_ty out_tm out_ty
-              H_tm H_ty H_var_eq H_stmts_ty =>
-      subst_vars
-      cases H_tm
-      cases letList_ty with
-      | nil => contradiction
-      | cons stmt_ty rst_stmts_ty =>
-      exists (ty_tenExp.letList rst_stmts_ty out_ty)
-      apply And.intro
-      . apply has_ty_tenExp.letList <;> try rfl
-        apply H_var_eq
-        cases H_stmts_ty with
-        | intro left right => apply right
-      . 
-      unfold has_ty_stmtLst at H_stmts_ty
-      simp at H_stmts_ty
-      
+def exp_suf_update (suf : Nat) : exp → exp
+  | exp.const c => exp.const c
+  | exp.binOp p1 var1 op
+               p2 var2 =>
+    exp.binOp p1 (var_suf_incr var1 suf) op
+               p2 (var_suf_incr var2 suf)
+  | exp.uniOp p f var =>
+    exp.uniOp p f (var_suf_incr var suf)
+  | exp.binTenSum indLst1 indLst2 indLst3
+                   p var1 var2 =>
+    exp.binTenSum indLst1 indLst2 indLst3 p
+                   (var_suf_incr var1 suf) (var_suf_incr var2 suf)
+  | exp.uniTenSum indLst1 indLst2 p var =>
+    exp.uniTenSum indLst1 indLst2 p (var_suf_incr var suf)
+def suf_update suf 
+  | tenStmt.stmt varLHS (unitTenExp.var varRHS) =>
+    tenStmt.stmt (var_suf_incr varLHS suf) (unitTenExp.var (var_suf_incr varRHS suf))
+  | tenStmt.stmt svar (unitTenExp.gen indList e) =>
+    tenStmt.stmt (var_suf_incr svar suf) (unitTenExp.gen indList (exp_suf_update suf e))
+  | tenStmt.stmt svar (unitTenExp.val val) =>
+    tenStmt.stmt svar (unitTenExp.val val)
+  | tenStmt.skip => tenStmt.skip
+def inline_one_prim target_var arg_vars var_suf
+  | tenFunc.func inp_vars (tenExp.letList fstmts out) =>
+      subst_lst_gen inp_vars arg_vars var_suf ++
+      (List.map (suf_update var_suf) fstmts) ++
+      [tenStmt.stmt target_var (unitTenExp.var (var_suf_incr out var_suf))]
+def inline_prims stmts (env : String → tenFunc) (var_suf : Nat) :=
+  match stmts with
+  | [] => []
+  | jStmt.stmt target_var prim_name diff_level arg_vars :: rst =>
+    let diffed_prog := forward_many_diff (env prim_name) diff_level
+    (inline_one_prim target_var arg_vars var_suf diffed_prog) ++ 
+      inline_prims rst env (1 + var_suf)
+  | jStmt.skip :: rst => tenStmt.skip :: inline_prims rst env var_suf
+/- transform a jaxpr into an ATL, by inlining primitives from environment -/
+def body_trans env body :=
+  match body with
+  | jaxpr_body.letList stmts out_var =>
+    tenExp.letList (inline_prims stmts env 1) out_var
+def jax_to_ATL p env :=
+  match p with
+  | jaxpr.func inp_vars body => 
+    tenFunc.func inp_vars (body_trans env body)
 
-| letList : ∀ letList_tm letList_ty tm_lst ty_lst out_tm out_ty,
-  letList_tm = tenExp.letList tm_lst out_tm →
-  letList_ty = ty_tenExp.letList ty_lst out_ty →
-  svar_eq out_tm out_ty = true →
-  has_ty_stmtLst tm_lst ty_lst → 
-  has_ty_tenExp letList_tm letList_ty
+def eval_prog prog args fenv :=
+  match jax_to_ATL prog fenv with
+  | tenFunc.func inp_vars (tenExp.letList stmts out) =>
+    (eval_stmts (inp_vars !->s* args ; empty_senv) stmts) out
 
+/- ********************* Library Functions **************************** -/
+inductive exp  
+| binTenSum : 
+  List Nat → List Nat → List Nat →
+  pred → stmt_var → stmt_var → exp
+| uniTenSum :
+  List Nat → List Nat →
+  pred → stmt_var → exp
 
-  | stp_stmts env env' stmt new_stmt some_stmts H_stp_stmt => 
-      
-  
-    
+notation "c:" c:60 => exp.const c
 
+notation "〚" pred1:70 "〛" var1:70 "+" "〚" pred2:70 "〛" var2:70 =>
+  (exp.binOp pred1 (stmt_var.stmtV var1 0) binPrim.add pred2 (stmt_var.stmtV var2 0))
+notation "〚" pred1:70 "〛" var1:70 "-" "〚" pred2:70 "〛" var2:70 =>
+  (exp.binOp pred1 (stmt_var.stmtV var1 0) binPrim.sub pred2 (stmt_var.stmtV var2 0))
+notation "〚" pred1:70 "〛" var1:70 "*" "〚" pred2:70 "〛" var2:70 =>
+  (exp.binOp pred1 (stmt_var.stmtV var1 0) binPrim.mult pred2 (stmt_var.stmtV var2 0))
+notation "〚" pred1:70 "〛" var1:70 "/" "〚" pred2:70 "〛" var2:70 =>
+  (exp.binOp pred1 (stmt_var.stmtV var1 0) binPrim.div pred2 (stmt_var.stmtV var2 0))
 
-  cases tm with
-  | letList stmts out =>
-  cases ty with
-  | letList stmts_ty out_ty =>
-  cases stmts with
-  | nil => contradiction
-  | cons stmt rst_stmts =>
-  cases stmts_ty with
-  | nil => contradiction
-  | cons stmt_ty rst_stmts_ty =>
-  cases stmt with
-  | skip =>
-    cases stmt_ty with
-    | skip => 
-      exists (ty_tenExp.letList rst_stmts_ty out_ty)
-      apply And.intro
-      . 
-    | stmt var exp_ty =>
-  | stmt var exp =>
-    cases stmt_ty with
-    | skip =>
-    | stmt var_ty exp_ty =>
-       
-      
-  cases H_step with
-  | stp_letList env env' stmts stmts' out H_stp_stmts =>
-    cases H_stp_stmts with
-    | stp_stmts env env' stmt new_stmt some_stmts H_stp_stmt => 
-      
-    | stp_skip env some_stmts=> 
-    
-    
-stp_stmts : ∀ env new_env stmt new_stmt some_stmts,
-| stp_skip : step_stmts (env, tenStmt.skip :: some_stmts) (env, some_stmts)
-| stp_stmts : ∀ env new_env stmt,
-  step_stmt (env, stmt) (new_env, new_stmt) →
-  step_stmts (env, stmt :: some_stmts) (new_env, new_stmt :: some_stmts)
+notation "uni:" "〚" pred:70 "〛" "-" var:70 =>
+  (exp.uniOp pred uniPrim.neg var)
 
+notation name:60 "←" ind_lst:60 "⊞" exp:60 ";" stmt_lst:60 =>
+  (tenStmt.stmt (stmt_var.stmtV name 0) (unitTenExp.gen ind_lst exp))
+  :: stmt_lst
 
-: ∀ env new_env stmts new_stmts out,
-  step_stmts (env,stmts) (new_env, new_stmts) →
-  step_fun_body (env, tenExp.letList stmts out) (new_env, tenExp.letList new_stmts out) 
-/- ********************* Example  **************************** -/
-notation (name := var_name) "!" name:arg => stmt_var.stmtV name 0
+notation var1:60 "←" var2:60 ";" stmt_lst:60 =>
+  (tenStmt.stmt (stmt_var.stmtV var1 0) (unitTenExp.var (stmt_var.stmtV var2 0)))
+  :: stmt_lst
+
+notation name:60 "←" ind_lst:60 exp:60 =>
+  name ← ind_lst ⊞ exp ; []
+
+notation var1:60 "←" var2:60 =>
+  var1 ← var2 ; []
+
+notation "inp_vars:" inp_var_lst:70 "body:" body_stmts:70 "return:" out:70 =>
+  tenFunc.func
+    (List.map (fun x => stmt_var.stmtV x 0) inp_var_lst)
+    (tenExp.letList body_stmts (stmt_var.stmtV out 0))
+
+def forty_two :=
+  inp_vars: ["x", "y"]
+  body: "x" ← [] ⊞ c: 42 ;
+        "out" ← "x"
+  return: "out"
+
+def tensor_add :=
+  inp_vars: ["x", "y"]
+  body: "x" ← [] ⊞ 〚pred.true〛 "x" + 〚pred.true〛 "y" ;
+        "out" ← "x"
+  return: "out"
+/- ********************* Example **************************** -/
+
+notation name:60 "←" func_name:60 ":" var_lst:60 ";" stmt_lst:61 =>
+  (jStmt.stmt 
+    (stmt_var.stmtV name 0) 
+    func_name
+    (List.map (fun x => stmt_var.stmtV x 0) var_lst))
+  :: stmt_lst
+notation name:60 "←" func_name:60 ":" var_lst:60 =>
+  name ← func_name : var_lst ; []
+
+notation "jaxpr:" inp_var_lst:70 "body:" body_stmts:70 "return:" out:70 =>
+  jaxpr.func
+    (List.map (fun x => stmt_var.stmtV x 0) inp_var_lst)
+    (jaxpr_body.letList body_stmts (stmt_var.stmtV out 0))
+
 
 def simple_prog :=
-  jaxpr.func [!"x", !"y", !"z"]
-  (jaxpr_body.letList 
-    [(! "a", "add", [!"x",  !"y"]), 
-    (!"b", "add", [! "a",  !"z"])] 
-    (!"b"))
+  jaxpr: ["x", "y", "z"]
+  body:
+    "a" ← "add" : ["x", "y"] ;
+    "b" ← "add" : ["a", "z"]
+  return: "b"
 def add_func :=
   let p := pred.true
   let X1 := stmt_var.stmtV (!"x")
@@ -827,7 +1272,7 @@ theorem eg : eval_prog simple_prog [arg1,arg2,arg3] prim_env =
  simp
  unfold exp_suf_update
  simp
- unfold var_suf_set
+ unfold var_suf_incr
  simp
  unfold subst_lst_gen subst_lst_gen subst_lst_gen
  simp
